vale/code/arch/x64/X64.Bytes_Semantics.fsti
@@ -1,5 +1,6 @@
 module X64.Bytes_Semantics
 
+module TS = X64.Taint_Semantics_s
 open X64.Bytes_Semantics_s
 open X64.Machine_s
 open Words_s
@@ -25,15 +26,19 @@ val same_mem_get_heap_val32 (ptr:int) (mem1 mem2:heap) : Lemma
   (requires get_heap_val32 ptr mem1 == get_heap_val32 ptr mem2)
   (ensures forall i. i >= ptr /\ i < ptr + 4 ==> mem1.[i] == mem2.[i])
 
-val frame_update_heap128 (ptr:int) (v:quad32) (s:state) : Lemma (
-  let s' = update_mem128 ptr v s in
+val frame_update_heap128 (ptr:int) (v:quad32) (mem:heap) : Lemma (
+  let mem' = update_heap128 ptr v mem in
   forall j. j < ptr \/ j >= ptr + 16 ==>
-    s.mem.[j] == s'.mem.[j])
+    mem.[j] == mem'.[j])
 
-val correct_update_get128 (ptr:int) (v:quad32) (s:state) : Lemma (
-  eval_mem128 ptr (update_mem128 ptr v s) == v)
-  [SMTPat (eval_mem128 ptr (update_mem128 ptr v s))]
+val correct_update_get128 (ptr:int) (v:quad32) (mem:heap) : Lemma (
+  get_heap_val128 ptr (update_heap128 ptr v mem) == v)
+  [SMTPat (get_heap_val128 ptr (update_heap128 ptr v mem))]
 
 val same_domain_update128 (ptr:int) (v:quad32) (mem:heap) : Lemma
   (requires valid_addr128 ptr mem)
   (ensures Map.domain mem == Map.domain (update_heap128 ptr v mem))
+
+val eval_ins_domains (ins:TS.tainted_ins) (s0:TS.traceState) : Lemma
+  (let s1 = TS.taint_eval_ins ins s0 in
+  Set.equal (Map.domain s0.TS.state.mem) (Map.domain s1.TS.state.mem))
