vale/code/arch/x64/X64.Memory_s.fst
@@ -121,9 +121,20 @@ let valid_state s = s.state.S.mem == I.down_mem s.mem.hs s.mem.addrs s.mem.ptrs
 
 let frame_valid s = ()
 
+let same_domain h m = Set.equal (I.addrs_set h.ptrs h.addrs) (Map.domain m)
+
+let lemma_same_domains h m1 m2 = ()
+
 let get_heap h = I.down_mem h.hs h.addrs h.ptrs
 
 let same_heap s1 s2 = ()
+
+let get_hs h m = 
+  {h with hs = I.up_mem m h.addrs h.ptrs h.hs}
+
+let get_hs_heap h = I.down_up_identity h.hs h.addrs h.ptrs
+
+let get_heap_hs m h = admit()
 
 let buffer_addr #t b h =
   let addrs = h.addrs in
@@ -1009,9 +1020,12 @@ let in_bounds64 (h:mem) (b:buffer64) (i:nat{i < buffer_length b}) : Lemma
   length_t_eq (TBase TUInt64) b;
   ()
 
-let bytes_valid ptr s =
+val bytes_valid_aux: (ptr:int) -> (h:mem) -> Lemma
+  (requires valid_mem64 ptr h)
+  (ensures S.valid_addr64 ptr (get_heap h))
+
+let bytes_valid_aux ptr h =
   let t = TBase TUInt64 in
-  let h = s.mem in
   let b = get_addr_ptr t ptr h h.ptrs in
   let i = get_addr_in_ptr t (buffer_length b) (buffer_addr b h) ptr 0 in
   in_bounds64 h b i;
@@ -1025,26 +1039,40 @@ let bytes_valid ptr s =
   I.addrs_set_mem h.ptrs b h.addrs (ptr+7);
   ()
 
-let valid_state_store_mem64 i v (s:state) =
-  if not (valid_mem64 i s.mem) then ()
-  else
-    let s' = S.update_mem i v s.state in
-    let h1 = store_mem_aux (TBase TUInt64) i s.mem.ptrs v s.mem in
-    let s' = {s with state = s'; mem = h1} in
-    store_buffer_aux_down64_mem i v s.mem;
-    store_buffer_aux_down64_mem2 i v s.mem;
-    let mem1 = s'.state.S.mem in
-    let mem2 = I.down_mem s'.mem.hs s.mem.addrs s.mem.ptrs in
+let bytes_valid ptr s = bytes_valid_aux ptr s.mem
+
+val valid_state_store_mem64_aux: (i:int) -> (v:nat64) -> (h:mem) -> Lemma 
+  (requires valid_mem64 i h)
+  (ensures (
+    let heap = get_heap h in
+    let heap' = S.update_heap64 i v heap in
+    let h' = store_mem64 i v h in
+    heap' == I.down_mem h'.hs h'.addrs h'.ptrs 
+  ))
+
+let valid_state_store_mem64_aux i v h =
+  let heap = get_heap h in
+  let heap' = S.update_heap64 i v heap in
+  let h1 = store_mem_aux (TBase TUInt64) i h.ptrs v h in
+  store_buffer_aux_down64_mem i v h;
+  store_buffer_aux_down64_mem2 i v h;
+  let mem1 = heap' in
+  let mem2 = I.down_mem h1.hs h.addrs h.ptrs in
+  let aux () : Lemma (forall j. mem1.[j] == mem2.[j]) =
     Bytes_Semantics.same_mem_get_heap_val i mem1 mem2;
-    Bytes_Semantics.correct_update_get i v s.state.S.mem;
-    Bytes_Semantics.frame_update_heap i v s.state.S.mem;
-    bytes_valid i s;
-    Bytes_Semantics.same_domain_update i v s.state.S.mem;
-    assert (forall j. mem1.[j] == mem2.[j]);
-    assert (Map.equal mem1 mem2);
-    ()
+    Bytes_Semantics.correct_update_get i v heap;
+    Bytes_Semantics.frame_update_heap i v heap
+  in let aux2 () : Lemma (Set.equal (Map.domain mem1) (Map.domain mem2)) =
+    bytes_valid_aux i h;
+    Bytes_Semantics.same_domain_update i v heap
+  in aux(); aux2();
+  Map.lemma_equal_intro mem1 mem2;
+  ()
 
-
+let valid_state_store_mem64 i v (s:state) = 
+  if not (valid_mem64 i s.mem) then ()
+  else valid_state_store_mem64_aux i v s.mem
+  
 val same_mem_get_heap_val128 (b:buffer128)
                           (i:nat{i < buffer_length b})
                           (v:quad32)
@@ -1245,9 +1273,12 @@ let in_bounds128 (h:mem) (b:buffer128) (i:nat{i < buffer_length b}) : Lemma
   length_t_eq (TBase TUInt128) b;
   ()
 
-let bytes_valid128 ptr s =
+val bytes_valid128_aux: (ptr:int) -> (h:mem) -> Lemma
+  (requires valid_mem128 ptr h)
+  (ensures S.valid_addr128 ptr (get_heap h))
+
+let bytes_valid128_aux ptr h =
   let t = TBase TUInt128 in
-  let h = s.mem in
   let b = get_addr_ptr t ptr h h.ptrs in
   let i = get_addr_in_ptr t (buffer_length b) (buffer_addr b h) ptr 0 in
   in_bounds128 h b i;
@@ -1269,51 +1300,134 @@ let bytes_valid128 ptr s =
   I.addrs_set_mem h.ptrs b h.addrs (ptr+15);
   ()
 
-let valid_state_store_mem128 i v (s:state) =
-  if not (valid_mem128 i s.mem) then ()
-  else
-    let s' = S.update_mem128 i v s.state in
-    let h1 = store_mem_aux (TBase TUInt128) i s.mem.ptrs v s.mem in
-    let s' = {s with state = s'; mem = h1} in
-    store_buffer_aux_down128_mem i v s.mem;
-    store_buffer_aux_down128_mem2 i v s.mem;
-    let mem1 = s'.state.S.mem in
-    let mem2 = I.down_mem s'.mem.hs s.mem.addrs s.mem.ptrs in
-    Bytes_Semantics.correct_update_get128 i v s.state;
+let bytes_valid128 ptr s = bytes_valid128_aux ptr s.mem
+
+val valid_state_store_mem128_aux: (i:int) -> (v:quad32) -> (h:mem) -> Lemma 
+  (requires valid_mem128 i h)
+  (ensures (
+    let heap = get_heap h in
+    let heap' = S.update_heap128 i v heap in
+    let h' = store_mem128 i v h in
+    heap' == I.down_mem h'.hs h'.addrs h'.ptrs 
+  ))
+
+let valid_state_store_mem128_aux i v h =
+  let heap = get_heap h in
+  let heap' = S.update_heap128 i v heap in
+  let h1 = store_mem_aux (TBase TUInt128) i h.ptrs v h in
+  store_buffer_aux_down128_mem i v h;
+  store_buffer_aux_down128_mem2 i v h;
+  let mem1 = heap' in
+  let mem2 = I.down_mem h1.hs h.addrs h.ptrs in
+  let aux () : Lemma (forall j. mem1.[j] == mem2.[j]) =
+    Bytes_Semantics.correct_update_get128 i v heap;
+    Opaque_s.reveal_opaque Bytes_Semantics_s.get_heap_val128_def;
     Bytes_Semantics.same_mem_get_heap_val32 i mem1 mem2;
     Bytes_Semantics.same_mem_get_heap_val32 (i+4) mem1 mem2;
     Bytes_Semantics.same_mem_get_heap_val32 (i+8) mem1 mem2;
     Bytes_Semantics.same_mem_get_heap_val32 (i+12) mem1 mem2;
-    Bytes_Semantics.frame_update_heap128 i v s.state;
-    bytes_valid128 i s;
-    Bytes_Semantics.same_domain_update128 i v s.state.S.mem;
-    assert (Map.equal mem1 mem2);
-    ()
+    Bytes_Semantics.frame_update_heap128 i v heap
+  in
+  let aux2 () : Lemma (Set.equal (Map.domain mem1) (Map.domain mem2)) =
+    bytes_valid128_aux i h;
+    Bytes_Semantics.same_domain_update128 i v heap
+  in aux (); aux2 ();
+  Map.lemma_equal_intro mem1 mem2
 
-let equiv_load_mem ptr s =
+let valid_state_store_mem128 i v (s:state) =
+  if not (valid_mem128 i s.mem) then ()
+  else valid_state_store_mem128_aux i v s.mem
+
+val equiv_load_mem_aux: (ptr:int) -> (h:mem) -> Lemma
+  (requires valid_mem64 ptr h)
+  (ensures load_mem64 ptr h == S.get_heap_val64 ptr (get_heap h))
+
+let equiv_load_mem_aux ptr h =
   let t = TBase TUInt64 in
-  let h = s.mem in
   let b = get_addr_ptr t ptr h h.ptrs in
   let i = get_addr_in_ptr t (buffer_length b) (buffer_addr b h) ptr 0 in
   let addr = buffer_addr b h in
   let contents = B.as_seq h.hs b in
-  let heap = s.state.S.mem in
+  let heap = get_heap h in
   index64_get_heap_val64 h b heap i;
-  lemma_load_mem64 b i h;
-  ()
+  lemma_load_mem64 b i h
 
+let equiv_load_mem ptr s = equiv_load_mem_aux ptr s.mem
 
-let equiv_load_mem128 ptr s =
+val equiv_load_mem128_aux: (ptr:int) -> (h:mem) -> Lemma
+  (requires valid_mem128 ptr h)
+  (ensures load_mem128 ptr h == S.get_heap_val128 ptr (get_heap h))
+
+let equiv_load_mem128_aux ptr h =
   let t = TBase TUInt128 in
-  let h = s.mem in
   let b = get_addr_ptr t ptr h h.ptrs in
   let i = get_addr_in_ptr t (buffer_length b) (buffer_addr b h) ptr 0 in
   let addr = buffer_addr b h in
   let contents = B.as_seq h.hs b in
-  let heap = s.state.S.mem in
+  let heap = get_heap h in
+  Opaque_s.reveal_opaque S.get_heap_val128_def;
   index128_get_heap_val128 h b heap i;
+  lemma_load_mem128 b i h
+
+let equiv_load_mem128 ptr s = equiv_load_mem128_aux ptr s.mem
+
+let low_lemma_valid_mem64 b i h = 
+  lemma_valid_mem64 b i h;
+  bytes_valid_aux (buffer_addr b h + 8 `op_Multiply` i) h
+
+let low_lemma_load_mem64 b i h =
+  lemma_valid_mem64 b i h;
+  lemma_load_mem64 b i h;
+  equiv_load_mem_aux (buffer_addr b h + 8 `op_Multiply` i) h
+
+val valid_state_store_mem64_aux2: (i:int) -> (v:nat64) -> (h:mem) -> Lemma 
+  (requires valid_mem64 i h)
+  (ensures (
+    let heap = get_heap h in
+    let heap' = S.update_heap64 i v heap in
+    let h' = store_mem64 i v h in
+    bytes_valid_aux i h;
+    X64.Bytes_Semantics.same_domain_update i v heap;
+    get_hs h heap' == h'
+  ))
+
+let valid_state_store_mem64_aux2 i v h =
+  valid_state_store_mem64_aux i v h;
+  let heap = get_heap h in
+  let heap' = S.update_heap64 i v heap in
+  let h' = store_mem64 i v h in
+  assert (    heap' == I.down_mem h'.hs h'.addrs h'.ptrs );
+  I.down_up_identity h'.hs h'.addrs h'.ptrs;
+  assert (get_hs h' heap' == h');
+  admit()
+
+
+let same_domain_update64 b i v h =
+  low_lemma_valid_mem64 b i h;
+  X64.Bytes_Semantics.same_domain_update (buffer_addr b h + 8 `op_Multiply` i) v (get_heap h)
+
+let low_lemma_store_mem64 b i v h =
+  lemma_valid_mem64 b i h;
+  lemma_store_mem64 b i v h;
+  valid_state_store_mem64_aux2 (buffer_addr b h + 8 `op_Multiply` i) v h
+  // let heap' = S.update_heap64 (buffer_addr b h + 8 `op_Multiply` i) v (get_heap h) in
+  // let h' = store_mem64 (buffer_addr b h + 8 `op_Multiply` i) v h in
+  // assume (get_hs h heap' == store_mem64 (buffer_addr b h + 8 `op_Multiply` i) v h)
+
+let low_lemma_valid_mem128 b i h =
+  lemma_valid_mem128 b i h;
+  bytes_valid128_aux (buffer_addr b h + 16 `op_Multiply` i) h
+
+let low_lemma_load_mem128 b i h =
+  lemma_valid_mem128 b i h;
   lemma_load_mem128 b i h;
-  ()
+  equiv_load_mem128_aux (buffer_addr b h + 16 `op_Multiply` i) h  
+
+let same_domain_update128 b i v h =
+  low_lemma_valid_mem128 b i h;
+  X64.Bytes_Semantics.same_domain_update128 (buffer_addr b h + 16 `op_Multiply` i) v (get_heap h)
+
+let low_lemma_store_mem128 b i v h = admit()
 
 let valid128_64 ptr h =
   let b = get_addr_ptr (TBase TUInt128) ptr h h.ptrs in
