vale/code/arch/x64/Interop.fsti
@@ -1,0 +1,123 @@
+module Interop
+
+module List = FStar.List.Tot.Base
+module HS = FStar.Monotonic.HyperStack
+module HH = FStar.Monotonic.HyperHeap
+module B = LowStar.Buffer
+module M = LowStar.Modifies
+module S8 = SecretByte
+
+open Opaque_s
+open X64.Machine_s
+open X64.Bytes_Semantics_s
+open X64.Bytes_Semantics
+
+let op_String_Access = Map.sel
+let op_String_Assignment = Map.upd
+
+inline_for_extraction
+let b8 = B.buffer UInt8.t
+let s8 = B.buffer S8.t
+
+let sub l i = l - i
+
+let rec loc_locs_disjoint_rec (l:s8) (ls:list s8) : Type0 =
+  match ls with
+  | [] -> True
+  | h::t -> M.loc_disjoint (M.loc_buffer l) (M.loc_buffer h) /\ loc_locs_disjoint_rec l t
+
+let rec locs_disjoint_rec (ls:list s8) : Type0 =
+  match ls with
+  | [] -> True
+  | h::t -> loc_locs_disjoint_rec h t /\ locs_disjoint_rec t
+
+unfold
+let bufs_disjoint (ls:list s8) : Type0 =
+  norm [iota; zeta; delta; delta_only [`%loc_locs_disjoint_rec;
+                                       `%locs_disjoint_rec]] (locs_disjoint_rec ls)
+
+unfold
+let buf_disjoint_from (b:s8) (ls:list s8) : Type0 =
+  norm [iota; zeta; delta; delta_only [`%loc_locs_disjoint_rec;
+                                       `%locs_disjoint_rec]] (loc_locs_disjoint_rec b ls)
+
+unfold
+let disjoint (#a:Type0) (ptr1 ptr2:B.buffer a) = M.loc_disjoint (M.loc_buffer ptr1) (M.loc_buffer ptr2)
+
+unfold
+let disjoint_or_eq ptr1 ptr2 = disjoint ptr1 ptr2 \/ ptr1 == ptr2
+
+let list_disjoint_or_eq (#a:Type0) (ptrs:list (B.buffer a)) =
+  forall p1 p2. List.memP p1 ptrs /\ List.memP p2 ptrs ==> disjoint_or_eq p1 p2
+
+let disjoint_addr addr1 length1 addr2 length2 =
+  (* The first buffer is completely before the second, or the opposite *)
+  addr1 + length1 < addr2 || addr2 + length2 < addr1
+
+type addr_map = (m:(b8 -> nat64){
+  (forall (buf1 buf2:b8). disjoint buf1 buf2 ==> 
+    disjoint_addr (m buf1) (B.length buf1) (m buf2) (B.length buf2)) /\
+  (forall (b:b8). m b + B.length b < pow2_64)})
+
+unfold
+let list_live (#a:Type0) mem (ptrs:list (B.buffer a)) = forall p . List.memP p ptrs ==> B.live mem p
+
+let correct_down_p (mem:HS.mem) (addrs:addr_map) (heap:heap) (p:b8) =
+  let length = B.length p in
+  let contents = B.as_seq mem p in
+  let addr = addrs p in
+  (forall i.  0 <= i /\ i < length ==> heap.[addr + i] == UInt8.v (FStar.Seq.index contents i))
+
+val addrs_set: (ptrs:list b8) -> (addrs:addr_map) -> GTot (s:Set.set int{
+  forall x. not (Set.mem x s) <==> 
+    (forall (b:b8{List.memP b ptrs}). x < addrs b \/ x >= addrs b + B.length b)})
+    
+val addrs_set_lemma: (ptrs1:list b8) -> (ptrs2:list b8) ->
+  (addrs:addr_map) -> Lemma
+  (requires forall b. List.memP b ptrs1 <==> List.memP b ptrs2)
+  (ensures addrs_set ptrs1 addrs == addrs_set ptrs2 addrs)
+
+val addrs_set_concat: (ptrs:list b8) -> (a:b8) ->
+  (addrs:addr_map) -> Lemma
+  (addrs_set (a::ptrs) addrs == Set.union (addrs_set ptrs addrs) (addrs_set [a] addrs))
+  
+val addrs_set_mem: (ptrs:list b8) -> (a:b8) ->
+  (addrs:addr_map) -> (i:int) -> Lemma
+  (requires List.memP a ptrs /\ i >= addrs a /\ i < addrs a + B.length a)
+  (ensures Set.mem i (addrs_set ptrs addrs))
+  
+let correct_down mem (addrs:addr_map) (ptrs: list b8) heap =
+  Set.equal (addrs_set ptrs addrs) (Map.domain heap) /\ 
+  (forall p. List.memP p ptrs ==> correct_down_p mem addrs heap p)
+
+(* Takes a Low* Hyperstack and a list of buffers and create a vale memory + keep track of the vale addresses *)
+val down_mem: (mem:HS.mem) -> (addrs: addr_map) -> (ptrs:list b8{list_disjoint_or_eq ptrs}) -> GTot (heap :heap {correct_down mem addrs ptrs heap})
+
+val same_unspecified_down: 
+  (mem1: HS.mem) -> 
+  (mem2: HS.mem) -> 
+  (addrs:addr_map) ->
+  (ptrs:list b8{list_disjoint_or_eq ptrs}) ->
+  Lemma (
+    let heap1 = down_mem mem1 addrs ptrs in
+    let heap2 = down_mem mem2 addrs ptrs in
+    forall i. (forall (b:b8{List.memP b ptrs}). 
+      let base = addrs b in
+      i < base \/ i >= base + B.length b) ==>
+      heap1.[i] == heap2.[i])
+
+val up_mem: 
+  (heap:heap) -> 
+  (addrs:addr_map) -> 
+  (ptrs: list b8{list_disjoint_or_eq ptrs}) -> 
+  (mem:HS.mem{list_live mem ptrs /\ Set.equal (addrs_set ptrs addrs) (Map.domain heap)}) -> 
+  GTot (new_mem:HS.mem{correct_down new_mem addrs ptrs heap /\ list_live new_mem ptrs})
+
+val down_up_identity: 
+  (mem:HS.mem) -> 
+  (addrs:addr_map) -> 
+  (ptrs:list b8{list_disjoint_or_eq ptrs /\ list_live mem ptrs }) -> 
+  Lemma (
+    let heap = down_mem mem addrs ptrs in 
+    let new_mem = up_mem heap addrs ptrs mem in
+    mem == new_mem)
