vale/code/arch/x64/X64.Vale.StateLemmas.fsti
@@ -2,21 +2,29 @@ module X64.Vale.StateLemmas
 open X64.Machine_s
 open X64.Vale.State
 open FStar.FunctionalExtensionality
-module S = X64.Semantics_s
 module BS = X64.Bytes_Semantics_s
 module ME = X64.Memory_s
 module TS = X64.Taint_Semantics_s
+open Prop_s
 
-unfold let ok' s = s.ME.state.BS.ok
-unfold let regs' s = s.ME.state.BS.regs
-unfold let xmms' s = s.ME.state.BS.xmms
-unfold let flags' s = s.ME.state.BS.flags
-unfold let mem' = ME.Mkstate'?.mem
+unfold let ok' s = s.BS.ok
+unfold let regs' s = s.BS.regs
+unfold let xmms' s = s.BS.xmms
+unfold let flags' s = s.BS.flags
+unfold let mem' s = s.BS.mem
 unfold let trace' = TS.MktraceState?.trace
 unfold let memTaint' = TS.MktraceState?.memTaint
 
-val state_to_S : s:state -> GTot TS.traceState
-val state_of_S : s:TS.traceState -> GTot state
+val same_domain: sv:state -> s:TS.traceState -> prop0
+
+val same_domain_eval_ins (c:TS.tainted_code{Ins? c}) (f:nat) (s0:TS.traceState) (sv:state) : Lemma
+  (requires same_domain sv s0)
+  (ensures (let s1 = TS.taint_eval_code c f s0 in
+     same_domain sv (Some?.v s1))
+  )
+
+val state_to_S : s:state -> GTot (s':TS.traceState{same_domain s s'})
+val state_of_S : sv:state -> (s:TS.traceState{same_domain sv s}) -> GTot state
 
 val lemma_to_ok : s:state -> Lemma
   (ensures s.ok == ok' (state_to_S s).TS.state)
@@ -26,9 +34,11 @@ val lemma_to_flags : s:state -> Lemma
   (ensures s.flags == flags' (state_to_S s).TS.state)
   [SMTPat s.flags]
 
+(*
 val lemma_to_mem : s:state -> Lemma
   (ensures s.mem === mem' (state_to_S s).TS.state)
   [SMTPat s.mem]
+*)
 
 val lemma_to_reg : s:state -> r:reg -> Lemma
   (ensures s.regs r == regs' (state_to_S s).TS.state r)
@@ -46,6 +56,7 @@ val lemma_to_memTaint : s:state -> Lemma
   (ensures s.memTaint === memTaint' (state_to_S s))
   [SMTPat s.memTaint]
 
+(*
 // No SMTPats for lemmas_of to avoid pattern loops
 val lemma_of_ok : s:TS.traceState -> Lemma
   (ensures (state_of_S s).ok == ok' s.TS.state)
@@ -64,25 +75,27 @@ val lemma_of_xmms : s:TS.traceState -> Lemma
 
 val lemma_of_memTaint : s:TS.traceState -> Lemma
   (ensures (state_of_S s).memTaint === memTaint' s)
+*)
 
 val lemma_to_eval_operand : s:state -> o:operand -> Lemma
-  (ensures eval_operand o s == S.eval_operand o (state_to_S s).TS.state)
+  (requires valid_operand o s)
+  (ensures eval_operand o s == BS.eval_operand o (state_to_S s).TS.state)
   [SMTPat (eval_operand o s)]
 
 val lemma_to_eval_xmm : s:state -> x:xmm -> Lemma
-  (ensures eval_xmm x s == S.eval_xmm x (state_to_S s).TS.state)
+  (ensures eval_xmm x s == BS.eval_xmm x (state_to_S s).TS.state)
   [SMTPat (eval_xmm x s)]
 
 val lemma_to_valid_operand : s:state -> o:operand -> Lemma
-  (ensures valid_operand o s ==> S.valid_operand o (state_to_S s).TS.state)
+  (ensures valid_operand o s ==> BS.valid_operand o (state_to_S s).TS.state)
   [SMTPat (valid_operand o s)]
 
 val lemma_of_to : s:state -> Lemma
-  (ensures s == state_of_S (state_to_S s))
-  [SMTPat (state_of_S (state_to_S s))]
+  (ensures s == state_of_S s (state_to_S s))
+  [SMTPat (state_of_S s (state_to_S s))]
 
-val lemma_to_of : s:TS.traceState -> Lemma
-  (ensures state_to_S (state_of_S s) == {s with TS.trace = []})
-  [SMTPat (state_to_S (state_of_S s))]
+val lemma_to_of : sv:state -> (s:TS.traceState{same_domain sv s}) -> Lemma
+  (ensures state_to_S (state_of_S sv s) == {s with TS.trace = []})
+  [SMTPat (state_to_S (state_of_S sv s))]
 
 unfold let op_String_Access (#a:eqtype) (#b:Type) (x:Map.t a b) (y:a) : Tot b = Map.sel x y
